converted Invariants.thy

Hoare/Invariants.thy
@@ -1,5 +1,5 @@
 theory Invariants
-imports "TrTermination"
+imports "TrTermination" "PathInvariant"
 begin
 
 definition basic_inv :: "global0 \<Rightarrow> bool" where
@@ -12,50 +12,25 @@ lemma orig_balance :
    total_balance (g_current g) < 2^256"
   using inv_orig_current by fastforce
 
+type_synonym 'a rel = "'a Relation.rel"
+
+definition tr :: "network \<Rightarrow> global0 rel" where
+"tr net = {(a,b) | a b. Continue b = next0 net (Continue a) }"
 
 lemma basic_invariant :
-  "Continue st2 = next0 net (Continue st1) \<Longrightarrow>
+  "(st1, st2) \<in> tr net \<Longrightarrow>
    basic_inv st1 \<Longrightarrow>
    basic_inv st2"
+apply (simp add:tr_def)
   by (metis basic_inv_def gas_next memu_next orig_balance tr_balance_continue tr_orig)
 
-definition re_invariant ::
-   "global0 \<Rightarrow> address \<Rightarrow> (w256 \<Rightarrow> storage \<Rightarrow> bool) \<Rightarrow> bool" where
-"re_invariant g addr iv = (
-  iv (account_balance0 (g_current g addr))
-     (account_storage0 (g_current g addr)) \<and>
-  (\<forall>x y s. iv x s \<longrightarrow> x < y \<longrightarrow> iv y s))"
-
-definition pop_action :: "contract_action \<Rightarrow> bool" where
-"pop_action act =
-   (act \<in> range ContractFail \<union> range ContractSuicide
-            \<union> range ContractReturn)"
-
-definition re_assumption ::
-  "network \<Rightarrow> address \<Rightarrow> program \<Rightarrow> (w256 \<Rightarrow> storage \<Rightarrow> bool) \<Rightarrow> bool" where
-"re_assumption net addr prog iv =
-  (\<forall>g args v1 h1.
-      g_vmstate g = InstructionToEnvironment (ContractCall args) v1 h1 \<longrightarrow>
-      callarg_recipient args = addr \<longrightarrow>
-      account_code0 (g_current g addr) = prog \<longrightarrow>
-  (\<exists>k g1 g2 g3 act2 v2 h2.
-      Unimplemented = iter_next net (Continue g) k \<or>
-      Continue g1 = next0 net (Continue g) \<and>
-      Continue g2 = iter_next net (Continue g) k \<and>
-      Continue g3 = iter_next net (Continue g) (Suc k) \<and>
-      g_vmstate g2 = InstructionToEnvironment act2 v2 h2 \<and>
-      pop_action act2 \<and>
-      g_stack g2 = g_stack g1 \<and>
-      re_invariant g3 addr iv))"
 
 (* call stack changes *)
 
 lemma stack_changes :
-  "Continue st2 = next0 net (Continue st1) \<Longrightarrow>
-   g_stack st2 = g_stack st1 \<or>
-   g_stack st2 = tl (g_stack st1) \<or>
-   tl (g_stack st2) = g_stack st1"
-by (auto simp add:next0_def Let_def
+  "(st1, st2) \<in> tr net \<Longrightarrow>
+   (g_stack st1, g_stack st2) \<in> push_pop"
+by (auto simp add:next0_def tr_def tlR_def push_pop_def Let_def
   split:if_split_asm option.split_asm list.split_asm
    contract_action.split_asm stack_hint.split_asm
    instruction_result.splits)
@@ -93,144 +68,110 @@ by (auto simp add:update_nonce_def transfer_balance_def
    add_balance_def sub_balance_def Let_def update_world_def)
 
 lemma exist_same :
-  "Continue st2 = next0 net (Continue st1) \<Longrightarrow>
+  "(st1, st2) \<in> tr net \<Longrightarrow>
    g_stack st2 = g_stack st1 \<Longrightarrow>
    account_exists (g_current st1 addr) =
    account_exists (g_current st2 addr)"
-by (auto simp add:next0_def Let_def
+by (auto simp add:next0_def Let_def tr_def
   exist_return
   split:if_split_asm option.split_asm list.split_asm
    contract_action.split_asm stack_hint.split_asm
    instruction_result.splits)
 
+(*
 lemma tl_wf : "(tl x22 = a # x22) = False"
 by (auto simp add:tl_def split:list.splits)
+*)
 
 lemma exist_push :
-  "Continue st2 = next0 net (Continue st1) \<Longrightarrow>
-   tl (g_stack st2) = g_stack st1 \<Longrightarrow>
+  "(st1, st2) \<in> tr net \<Longrightarrow>
+   (g_stack st2, g_stack st1) \<in> tlR \<Longrightarrow>
    account_exists (g_current st1 addr) \<Longrightarrow>
    account_exists (g_current st2 addr)"
-by (auto simp add:next0_def Let_def
+by (auto simp add:tr_def tlR_def next0_def Let_def
   exist_return exist_call exist_transfer
-  exist_update exist_nonce tl_wf
-  split:if_split_asm option.split_asm list.split_asm
-   contract_action.split_asm stack_hint.split_asm
-   instruction_result.splits)
-
-lemma exist_push2 :
-  "Continue st2 = next0 net (Continue st1) \<Longrightarrow>
-   g_stack st2 = (a,b,c,d) # g_stack st1 \<Longrightarrow>
-   account_exists (g_current st1 addr) \<Longrightarrow>
-   account_exists (a addr)"
-by (auto simp add:next0_def Let_def
-  exist_return exist_call exist_transfer
-  exist_update exist_nonce tl_wf
+  exist_update exist_nonce 
   split:if_split_asm option.split_asm list.split_asm
    contract_action.split_asm stack_hint.split_asm
    instruction_result.splits)
 
 lemma exist_pop :
-  "Continue st2 = next0 net (Continue st1) \<Longrightarrow>
-   g_stack st2 = (a,b,c,d) # g_stack st1 \<Longrightarrow>
-   account_exists (a addr) \<Longrightarrow>
-   account_exists (g_current st2 addr)"
-by (auto simp add:next0_def Let_def
-  exist_return exist_call exist_transfer
-  exist_update exist_nonce
-  split:if_split_asm option.split_asm list.split_asm
-   contract_action.split_asm stack_hint.split_asm
-   instruction_result.splits)
-
-lemma weird_current :
-  "st2 = st1
-       \<lparr>g_stack := b,
-        g_current := a,
-        g_cctx := c,
-        g_vmstate := d\<rparr> \<Longrightarrow>
-  g_current st2 = a"
-by auto
-
-lemma weird_weird_aux :
-  "(st2 = st1
-       \<lparr>g_stack := b,
-        g_current := a,
-        g_cctx := c,
-        g_vmstate := d\<rparr>) =
-    (st2 = \<lparr>
-        g_orig = g_orig st1,
-        g_stack = b,
-        g_current = a,
-        g_cctx = c,
-        g_killed = g_killed st1,
-        g_vmstate = d,
-        g_create = g_create st1
- \<rparr> )"
-by auto
-
-lemma weird_weird_aux2 :
-  "st1
-       \<lparr>g_stack := b,
-        g_current := a,
-        g_cctx := c,
-        g_vmstate := d\<rparr> =
-    \<lparr>
-        g_orig = g_orig (st1::global0),
-        g_stack = b,
-        g_current = a,
-        g_cctx = c,
-        g_killed = g_killed st1,
-        g_vmstate = d,
-        g_create = g_create st1
- \<rparr>"
-by auto
-
-
-lemma weird_weird :
-  "(st2 = (st1::global0)
-       \<lparr>g_stack := b,
-        g_current := a,
-        g_cctx := c,
-        g_vmstate := d\<rparr>) =
-  (g_current st2 = a \<and>
-   g_stack st2 = b \<and>
-   g_cctx st2 = c \<and>
-   g_vmstate st2 = d \<and>
-   g_orig st2 = g_orig st1 \<and>
-   g_create st2 = g_create st1 \<and>
-   g_killed st2 = g_killed st1 )"
-by auto
-
-lemma weird_weird2 :
-  "(st2 = (st1::global0)
-       \<lparr>g_stack := b,
-        g_current := a,
-        g_cctx := c,
-        g_vmstate := d,
-        g_killed := e \<rparr>) =
-  (g_current st2 = a \<and>
-   g_stack st2 = b \<and>
-   g_cctx st2 = c \<and>
-   g_vmstate st2 = d \<and>
-   g_orig st2 = g_orig st1 \<and>
-   g_create st2 = g_create st1 \<and>
-   g_killed st2 = e )"
-by auto
-
-lemma exist_pop2 :
-  "Continue st2 = next0 net (Continue st1) \<Longrightarrow>
-   (a,b,c,d) # g_stack st2 = g_stack st1 \<Longrightarrow>
+  "(st1, st2) \<in> tr net \<Longrightarrow>
+(*   (g_stack st1, g_stack st2) \<in> tlR \<Longrightarrow> *)
+   hd (g_stack st1) = (a,b,c,d)  \<Longrightarrow>
    account_exists (g_current st1 addr) \<Longrightarrow>
    account_exists (a addr) \<Longrightarrow>
    account_exists (g_current st2 addr)"
-by (auto simp add:next0_def Let_def
+by (auto simp add:next0_def Let_def tr_def tlR_def
   exist_return exist_call exist_transfer
-  exist_update exist_nonce weird_weird weird_weird2
+  exist_update exist_nonce (* weird_weird weird_weird2 *)
   create_account_def
   set_account_code_def
   split:if_split_asm option.split_asm list.split_asm
    contract_action.split_asm stack_hint.split_asm
    instruction_result.splits)
+
+
+lemma exist_push2 :
+  "(st1, st2) \<in> tr net \<Longrightarrow>
+   g_stack st2 = (a,b,c,d) # g_stack st1 \<Longrightarrow>
+   account_exists (g_current st1 addr) \<Longrightarrow>
+   account_exists (a addr)"
+by (auto simp add:next0_def Let_def
+  exist_return exist_call exist_transfer
+  exist_update exist_nonce tr_def
+  split:if_split_asm option.split_asm list.split_asm
+   contract_action.split_asm stack_hint.split_asm
+   instruction_result.splits)
+
+lemma exist_push3 :
+   "(st1, st2) \<in> tr net \<Longrightarrow>
+       g_stack st2 =
+       (a, aa, ab, b) # g_stack st1 \<Longrightarrow>
+       account_exists (a addr) \<Longrightarrow>
+       account_exists (g_current st2 addr)"
+by (auto simp add:next0_def Let_def
+  exist_return exist_call exist_transfer
+  exist_update exist_nonce tr_def
+  split:if_split_asm option.split_asm list.split_asm
+   contract_action.split_asm stack_hint.split_asm
+   instruction_result.splits)
+
+fun stack_hint :: "world_state * variable_ctx * constant_ctx * stack_hint \<Rightarrow> stack_hint" where
+"stack_hint (a,b,c,d) = d"
+
+fun stack_state :: "world_state * variable_ctx * constant_ctx * stack_hint \<Rightarrow> world_state" where
+"stack_state (a,b,c,d) = a"
+
+definition states_t :: "global0 \<Rightarrow> world_state * world_state list" where
+"states_t g = (g_current g, map stack_state (g_stack g))"
+
+lemma exist_mono :
+  "(st1, st2) \<in> tr net \<Longrightarrow>
+   (states_t st1, states_t st2) \<in> mono_rules
+      (\<lambda>st. account_exists (st addr))"
+apply (cases "g_stack st1 = g_stack st2")
+apply (subgoal_tac "(states_t st1, states_t st2)
+    \<in> mono_same (\<lambda>st. account_exists (st addr))")
+apply (simp add:mono_rules_def)
+apply (clarsimp simp add:mono_same_def states_t_def)
+  apply (simp add: exist_same)
+apply (cases "(g_stack st1,g_stack st2) \<in> tlR")
+apply (subgoal_tac "(states_t st1, states_t st2)
+    \<in> mono_pop (\<lambda>st. account_exists (st addr))")
+apply (simp add:mono_rules_def)
+apply (clarsimp simp add:mono_pop_def states_t_def tlR_def)
+  apply (simp add: exist_pop)
+apply (cases "(g_stack st2,g_stack st1) \<in> tlR")
+apply (subgoal_tac "(states_t st1, states_t st2)
+    \<in> mono_push (\<lambda>st. account_exists (st addr))")
+apply (simp add:mono_rules_def)
+apply (auto simp add:mono_push_def states_t_def tlR_def)
+  using exist_push2 apply blast
+  using exist_push3 apply blast
+using stack_changes [of st1 st2 net]
+apply (simp add:push_pop_def tlR_def)
+done
 
 
 lemma can_exit :
@@ -243,9 +184,9 @@ by (auto simp add:next0_def Let_def
    instruction_result.splits)
 
 lemma create_const :
-  "Continue st2 = next0 net (Continue st1) \<Longrightarrow>
+  "(st1, st2) \<in> tr net \<Longrightarrow>
    g_create st1 = g_create st2"
-by (auto simp add:next0_def Let_def
+by (auto simp add:next0_def Let_def tr_def
   split:if_split_asm option.split_asm list.split_asm
    contract_action.split_asm stack_hint.split_asm
    instruction_result.splits)
@@ -283,69 +224,50 @@ by (auto simp add:update_nonce_def transfer_balance_def
    add_balance_def sub_balance_def Let_def update_world_def)
 
 lemma code_stay :
-  "Continue st2 = next0 net (Continue st1) \<Longrightarrow>
+  "(st1, st2) \<in> tr net \<Longrightarrow>
    g_stack st2 = g_stack st1 \<Longrightarrow>
    account_code0 (g_current st1 addr) =
    account_code0 (g_current st2 addr)"
-by (auto simp add:next0_def Let_def
+by (auto simp add:next0_def Let_def tr_def
   code_return
   split:if_split_asm option.split_asm list.split_asm
    contract_action.split_asm stack_hint.split_asm
    instruction_result.splits)
-
-lemma weird : 
-   "g_current st2 = a \<Longrightarrow>
-    account_code0 (a addr) = account_code0 (g_current st2 addr)"
-by auto
-
-lemma weird2 :
- "st2 = st1
-    \<lparr>g_stack := d, g_current := a,
-       g_cctx := c,
-       g_vmstate := e \<rparr> \<Longrightarrow>
-  g_current st2 = a"
-by auto
 
 (* separate cases for fail etc. *)
 lemma code_fail :
-  "Continue st2 = next0 net (Continue st1) \<Longrightarrow>
+  "(st1, st2) \<in> tr net \<Longrightarrow>
    g_vmstate st1 = InstructionToEnvironment (ContractFail lst) v1 hint \<Longrightarrow>
-   (a,b,c,d) # g_stack st2 = g_stack st1 \<Longrightarrow>
+   hd (g_stack st1) = (a,b,c,d) \<Longrightarrow>
    account_code0 (a addr) =
    account_code0 (g_current st2 addr)"
-by (auto simp add:next0_def Let_def
+by (auto simp add:next0_def Let_def tr_def
   code_return
   split:if_split_asm option.split_asm list.split_asm
    contract_action.split_asm stack_hint.split_asm
    instruction_result.splits)
 
-fun stack_hint :: "world_state * variable_ctx * constant_ctx * stack_hint \<Rightarrow> stack_hint" where
-"stack_hint (a,b,c,d) = d"
-
-fun stack_state :: "world_state * variable_ctx * constant_ctx * stack_hint \<Rightarrow> world_state" where
-"stack_state (a,b,c,d) = a"
-
 lemma code_suicide :
-  "next0 net (Continue st1) = Continue st2 \<Longrightarrow>
+  "(st1, st2) \<in> tr net \<Longrightarrow>
    g_vmstate st1 = InstructionToEnvironment (ContractSuicide lst) v1 hint \<Longrightarrow>
    stack_hint (hd (g_stack st1)) \<noteq> CreateAddress addr \<Longrightarrow>
    account_code0 (g_current st1 addr) =
    account_code0 (g_current st2 addr)"
-by (auto simp add:next0_def Let_def
+by (auto simp add:next0_def Let_def tr_def
   code_return code_update create_account_def
   split:if_split_asm option.split_asm list.split_asm
    contract_action.split_asm stack_hint.split_asm
    instruction_result.splits)
 
 lemma code_ret :
-  "next0 net (Continue st1) = Continue st2 \<Longrightarrow>
+  "(st1, st2) \<in> tr net \<Longrightarrow>
    g_vmstate st1 = InstructionToEnvironment (ContractReturn lst) v1 hint \<Longrightarrow>
    stack_hint (hd (g_stack st1)) \<noteq> CreateAddress addr \<Longrightarrow>
    account_code0 (g_current st2 addr) =
    account_code0 (g_current st1 addr) \<or>
    account_code0 (g_current st2 addr) =
    account_code0 (stack_state (hd (g_stack st1)) addr)"
-by (auto simp add:next0_def Let_def
+by (auto simp add:next0_def Let_def tr_def
   code_return code_update create_account_def
   split:if_split_asm option.split_asm list.split_asm
    contract_action.split_asm stack_hint.split_asm
@@ -354,330 +276,75 @@ by (auto simp add:next0_def Let_def
 
 (* in the hypotheses, matters a lot if it is a=b or b=a *)
 lemma code_push :
-  "Continue st2 = next0 net (Continue st1) \<Longrightarrow>
-   tl (g_stack st2) = g_stack st1 \<Longrightarrow>
+  "(st1, st2) \<in> tr net \<Longrightarrow>
+   (g_stack st2, g_stack st1) \<in> tlR \<Longrightarrow>
    account_exists (g_current st1 addr) \<Longrightarrow>
    account_code0 (g_current st1 addr) =
    account_code0 (g_current st2 addr)"
-by (auto simp add:next0_def Let_def
-  code_return code_call code_transfer code_update tl_wf
+by (auto simp add:next0_def Let_def tr_def tlR_def
+  code_return code_call code_transfer code_update
   code_nonce
   split:if_split_asm option.split_asm list.split_asm
    contract_action.split_asm stack_hint.split_asm
    instruction_result.splits)
 
 lemma push_create_hint :
-  "Continue st2 = next0 net (Continue st1) \<Longrightarrow>
+  "(st1, st2) \<in> tr net \<Longrightarrow>
    g_stack st2 = abcd # g_stack st1 \<Longrightarrow>
    stack_hint abcd = CreateAddress addr \<Longrightarrow>
    account_exists (g_current st1 addr) \<Longrightarrow>
    False"
-by (auto simp add:next0_def Let_def
+by (auto simp add:next0_def Let_def tr_def
   code_return code_call
-  code_transfer code_update tl_wf
+  code_transfer code_update 
   code_nonce get_hint_def
   split:if_split_asm option.split_asm list.split_asm
    contract_action.split_asm stack_hint.split_asm
    instruction_result.splits)
 
-lemma iter_next_head :
-  "iter_next net (next0 net g) l = next0 net (iter_next net g l)"
-by (induction l arbitrary:g; auto)
+(* how to apply this with mono invariants? *)
 
-lemma continue_next :
- "Continue st2 = next0 net g \<Longrightarrow>
-  \<exists>st3. Continue st3 = g"
-by (auto simp add:next0_def Let_def
+definition create_exist_inv :: "address \<Rightarrow> global0 \<Rightarrow> bool" where
+"create_exist_inv addr g =
+   (\<forall>el \<in> set (g_stack g).
+          account_exists (stack_state el addr) \<longrightarrow>
+          stack_hint el \<noteq> CreateAddress addr)"
+
+lemma create_exist_inv_stay :
+  "g_stack st2 = g_stack st1 \<Longrightarrow>
+   create_exist_inv addr st1 \<Longrightarrow>
+   create_exist_inv addr st2"
+by (simp add:create_exist_inv_def)
+
+lemma create_exist_inv_pop :
+  "(g_stack st1, g_stack st2) \<in> tlR \<Longrightarrow>
+   create_exist_inv addr st1 \<Longrightarrow>
+   create_exist_inv addr st2"
+by (auto simp add:create_exist_inv_def tlR_def)
+
+lemma create_exist_inv_push :
+  "(st1, st2) \<in> tr net \<Longrightarrow>
+   g_stack st2 = abcd # g_stack st1 \<Longrightarrow>
+   create_exist_inv addr st1 \<Longrightarrow>
+   create_exist_inv addr st2"
+by (auto simp add:next0_def Let_def tr_def
+  code_return code_call create_exist_inv_def
+  code_transfer code_update 
+  code_nonce get_hint_def exist_nonce
   split:if_split_asm option.split_asm list.split_asm
    contract_action.split_asm stack_hint.split_asm
-   instruction_result.splits global_state.splits)
+   instruction_result.splits)
 
-lemma continues :
-   "Continue st2 = iter_next net g k \<Longrightarrow>
-    \<exists> st3. Continue st3 = g"
-apply (induction k arbitrary:g; auto)
-using continue_next
-  by blast
-
-lemma iter_next_add :
-  "iter_next net g (k+l) =
-   iter_next net (iter_next net g l) k"
-by (induction l arbitrary:g; auto)
-
-lemma continues2 :
-   "Continue st2 = iter_next net g (k+l) \<Longrightarrow>
-    \<exists> st3. Continue st3 = iter_next net g l"
-using continues and iter_next_add
-  by simp
-
-lemma continues3 :
-   "Continue st2 = iter_next net g k \<Longrightarrow>
-    l < k \<Longrightarrow>
-    \<exists> st3. Continue st3 = iter_next net g l"
-  by (metis add.commute less_imp_add_positive continues2)
-
-definition state_mono :: "(world_state \<Rightarrow> bool) \<Rightarrow> global0 \<Rightarrow> bool" where
-"state_mono iv g = (\<forall>i < length (states g)-1.
-   iv (states g!(i+1)) \<longrightarrow> iv (states g!i))"
-
-lemma mono_same :
-  "g_stack st2 = g_stack st1 \<Longrightarrow>
-   (iv (g_current st1) \<longrightarrow> iv (g_current st2)) \<Longrightarrow>
-   state_mono iv st1 \<Longrightarrow>
-   state_mono iv st2"
-apply (auto simp add:state_mono_def states_def)
-apply (case_tac "i"; auto)
-apply (case_tac "i"; auto)
-done
-
-lemma mono_push :
-  "g_stack st2 = (a,b,c,d) # g_stack st1 \<Longrightarrow>
-   ( iv (g_current st1) \<longrightarrow> iv a ) \<Longrightarrow>
-   ( iv a \<longrightarrow> iv (g_current st2) ) \<Longrightarrow>
-   state_mono iv st1 \<Longrightarrow>
-   state_mono iv st2"
-apply (auto simp add:state_mono_def states_def)
-apply (case_tac "i"; auto)
-apply (case_tac "nat"; auto)
-apply (case_tac "i"; auto)
-apply (case_tac "nat"; auto)
-apply (case_tac "i"; auto)
-apply (case_tac "nat"; auto)
-done
-
-lemma mono_simple_pop :
-  "g_stack st1 = (a,b,c,d) # g_stack st2 \<Longrightarrow>
-   g_current st2 = a \<Longrightarrow>
-   state_mono iv st1 \<Longrightarrow>
-   state_mono iv st2"
-by (auto simp add:state_mono_def states_def)
-
-lemma mono_pop2 :
-  "(a,b,c,d) # g_stack st2 = g_stack st1 \<Longrightarrow>
-   ( iv a \<longrightarrow> iv (g_current st2) ) \<Longrightarrow>
-   state_mono iv st1 \<Longrightarrow>
-   state_mono iv st2"
-apply (rule mono_same [of st2 "st2\<lparr>g_current := a\<rparr>" iv])
-apply simp
-apply simp
-using mono_simple_pop
-  by (metis (no_types, lifting) global0.select_convs(2) global0.select_convs(3) global0.surjective global0.update_convs(3))
-
-lemma mono_empty :
- "g_stack st2 = [] \<Longrightarrow> state_mono iv st2"
-by (auto simp add:state_mono_def states_def)
-
-lemma get_mono :
-  "state_mono iv st1 \<Longrightarrow>
-   g_stack st1 = (a, b, c, d) # rest \<Longrightarrow>
-   iv a \<Longrightarrow>
-   iv (g_current st1)"
-by (auto simp add:state_mono_def states_def)
-
-lemma exist_mono :
-  "Continue st2 = next0 net (Continue st1) \<Longrightarrow>
-   state_mono (\<lambda>st. account_exists (st addr)) st1 \<Longrightarrow> 
-   state_mono (\<lambda>st. account_exists (st addr)) st2"
-apply (cases "g_stack st2 = g_stack st1 \<or>
-   g_stack st2 = tl (g_stack st1) \<or>
-   tl (g_stack st2) = g_stack st1")
-defer
-using stack_changes apply force
-apply auto
-  using exist_same mono_same apply auto[1]
-apply (cases "g_stack st1"; auto simp:mono_empty)
-subgoal for a b c d
-apply (rule mono_pop2 [of a b c d st2 st1]; auto)
-using exist_pop2 [of st2 net st1 a b c d addr] get_mono
-apply force
-done
-apply (cases "g_stack st2"; auto simp:mono_empty)
-subgoal for a b c d
-apply (rule mono_push [of st2 a b c d st1]; auto)
-  using exist_push2 apply force
-  using exist_pop by auto
-done
-
-lemma imed_stack_length_aux :
-"   ( Continue st2 =
-           iter_next net (Continue st3) k \<Longrightarrow>
-           length (g_stack st3) \<le> l \<Longrightarrow>
-           l \<le> length (g_stack st2) \<Longrightarrow>
-           \<exists>st k2.
-              Continue st =
-              iter_next net (Continue st3) k2 \<and>
-              length (g_stack st) = l \<and>
-              k2 \<le> k ) \<Longrightarrow>
-       Continue st2 = iter_next net (Continue st1) (Suc k) \<Longrightarrow>
-       Continue st3 = next0 net (Continue st1) \<Longrightarrow>
-       length (g_stack st1) \<le> l \<Longrightarrow>
-       l \<le> length (g_stack st2) \<Longrightarrow>
-       \<exists>st k2.
-          Continue st =
-          iter_next net (Continue st1) k2 \<and>
-          length (g_stack st) = l \<and> k2 \<le> Suc k"
-apply (cases "g_stack st1 = g_stack st3")
-apply force
-apply (cases "g_stack st3 = tl (g_stack st1)")
-apply force
-apply (cases "g_stack st1 = tl (g_stack st3)")
-apply force
-
-using stack_changes
-apply fastforce
-done
-
-lemma imed_stack_length_aux2 :
-"  \<exists> st3. ( Continue st3 = next0 net (Continue st1) \<and>
-   ( Continue st2 =
-           iter_next net (Continue st3) k \<longrightarrow>
-           length (g_stack st3) \<le> l \<longrightarrow>
-           l \<le> length (g_stack st2) \<longrightarrow>
-           (\<exists>st k2.
-              Continue st =
-              iter_next net (Continue st3) k2 \<and>
-              length (g_stack st) = l \<and>
-              k2 \<le> k ))) \<Longrightarrow>
-       Continue st2 = iter_next net (Continue st1) (Suc k) \<Longrightarrow>
-       length (g_stack st1) \<le> l \<Longrightarrow>
-       l \<le> length (g_stack st2) \<Longrightarrow>
-       \<exists>st k2.
-          Continue st =
-          iter_next net (Continue st1) k2 \<and>
-          length (g_stack st) = l \<and> k2 \<le> Suc k"
-apply auto
-apply (rule imed_stack_length_aux; auto)
-apply (rule imed_stack_length_aux; auto)
-done
-
-lemma ex_and :
-"\<exists>st3. P st3 \<Longrightarrow>
- \<forall>st. (P st \<longrightarrow> Q st) \<Longrightarrow> 
- \<exists>st3. P st3 \<and> Q st3"
-by auto
-
-lemma imed_stack_length :
-  "Continue st2 = iter_next net (Continue st1) k \<Longrightarrow>
-   length (g_stack st1) \<le> l \<Longrightarrow>
-   l \<le> length (g_stack st2) \<Longrightarrow>
-   \<exists>st k2. Continue st = iter_next net (Continue st1) k2
-        \<and> length (g_stack st) = l \<and> k2 \<le> k"
-apply (induction k arbitrary:st1)
-apply simp
-apply (rule imed_stack_length_aux2 [of _ _ st2])
-apply auto
-using continues apply force
-done
-
-lemma next_unchanged :
-  "Continue st2 = next0 net (Continue st1) \<Longrightarrow>
-   l \<le> length (g_stack st2) \<Longrightarrow>
-   l \<le> length (g_stack st1) \<Longrightarrow>
-   take l (rev (g_stack st2)) = take l (rev (g_stack st1))"
-apply (cases "g_stack st1 = g_stack st2")
-apply force
-apply (cases "g_stack st2 = tl (g_stack st1)")
-apply auto
-  apply (smt One_nat_def add_diff_cancel_left diff_le_self drop_0 drop_Suc drop_drop drop_rev le_add_diff_inverse length_rev length_tl nat_add_left_cancel_le rev_swap take_rev)
-apply (cases "g_stack st1 = tl (g_stack st2)")
-apply auto
-  apply (smt One_nat_def add_diff_cancel_left add_le_cancel_left diff_le_self drop_0 drop_Suc drop_drop drop_rev le_add_diff_inverse length_rev length_tl rev_swap take_rev)
-using stack_changes
-apply fastforce
-done
-
-lemma stack_unchanged_split :
-  "Continue st2 = iter_next net (next0 net (Continue st1)) k \<Longrightarrow>
-   \<exists>st3. Continue st3 = next0 net (Continue st1) \<and>
-     (take l (rev (g_stack st2)) = take l (rev (g_stack st3)) \<and>
-     take l (rev (g_stack st3)) = take l (rev (g_stack st1))) \<Longrightarrow>
-   take l (rev (g_stack st2)) = take l (rev (g_stack st1))"
-by auto
-
-lemma helper :
-  "(\<And>st1. A1 (st1::global0) \<Longrightarrow> A2 st1 \<Longrightarrow> f x = f st1) \<Longrightarrow>
-    A1 st \<Longrightarrow> A2 st \<Longrightarrow> f x = f st"
-by auto
-
-lemma stack_unchanged :
-  "Continue st2 = iter_next net (Continue st1) k \<Longrightarrow>
-   (\<forall>sti. \<forall> k1 \<le> k.
-   Continue sti = iter_next net (Continue st1) k1 \<longrightarrow>
-   l \<le> length (g_stack sti) ) \<Longrightarrow>
-   take l (rev (g_stack st2)) = take l (rev (g_stack st1))"
-apply (induction k arbitrary:st1)
-apply simp
-apply auto
-subgoal for k st3
-apply (rule stack_unchanged_split)
-apply auto
-apply (rule ex_and)
-using continues apply force
-apply auto
-defer
-apply (rule next_unchanged)
-apply auto
-apply force
-apply force
-subgoal for st
-apply (rule helper [of "\<lambda>st1. iter_next net (next0 net (Continue st3)) k =
-        iter_next net (Continue st1) k"
-  "\<lambda>st1. \<forall>sti k1.
-           k1 \<le> k \<longrightarrow>
-           Continue sti =
-           iter_next net (Continue st1) k1 \<longrightarrow>
-           l \<le> length (g_stack sti)"])
-apply auto
-  by fastforce
-done done
-
-definition takeLast :: "nat \<Rightarrow> 'a list \<Rightarrow> 'a list" where
-"takeLast n lst = rev (take n (rev lst))"
-
-lemma takeLast_drop :
-  "takeLast n lst = drop (length lst - n) lst"
-apply (induction lst arbitrary:n)
-apply (auto simp add:takeLast_def)
-  by (metis length_Cons length_rev rev.simps(2) rev_append rev_rev_ident take_append take_rev)
-
-lemma find_stack :
-  "Continue st2 = iter_next net (Continue st1) k \<Longrightarrow>
-   length (g_stack st2) \<le> length (g_stack st1) \<Longrightarrow>
-   \<exists>k3 st3. Continue st3 = iter_next net (Continue st1) k3 \<and>
-   g_stack st3 = takeLast (length (g_stack st2)) (g_stack st1) \<and>
-   k3 \<le> k"
-
-
-(* account existence continues until first return *)
-
-definition first_return :: "network \<Rightarrow> nat \<Rightarrow> global0 \<Rightarrow> global0 \<Rightarrow> bool" where
-"first_return net k st st2 = (
-   (Continue st2 = iter_next net (Continue st) k \<and>
-          tl (g_stack st) = g_stack st2 \<and>
-    (\<forall>l<k. \<forall>st3. Continue st3 = iter_next net (Continue st) l \<longrightarrow>
-                 tl (g_stack st) \<noteq> g_stack st3)))"
-
-lemma stack_length_return :
-  "first_return net k st st3 \<Longrightarrow>
-   Continue st2 = iter_next net (Continue st1) k2 \<Longrightarrow>
-   length (g_stack st2) > length (g_stack st3)"
-
-lemma exist_until_return :
-  "account_exists (g_current st1 addr) \<Longrightarrow>
-   first_return net st1 k \<Longrightarrow>
-   l < k \<Longrightarrow>
-   Continue st3 = iter_next net (Continue st) l \<Longrightarrow>
-   account_exists (g_current st3 addr)"
 
 (* storage changes *)
 (* storage changes are first the same as code changes, but also from
    calls out *)
 lemma storage_continue :
-  "Continue st2 = next0 net (Continue st1) \<Longrightarrow>
+  "(st1, st2) \<in> tr net \<Longrightarrow>
    g_vmstate st1 \<in> range InstructionContinue \<Longrightarrow>
    account_storage0 (g_current st1 addr) =
    account_storage0 (g_current st2 addr)"
-by (auto simp add:next0_def Let_def
+by (auto simp add:next0_def Let_def tr_def
   split:if_split_asm option.split_asm list.split_asm
    contract_action.split_asm stack_hint.split_asm
    instruction_result.splits)
